theories/heap_lang/robust_safety.v
@@ -8,123 +8,511 @@ Import uPred.
 
 Local Hint Resolve to_of_val.
 
-(** * Adversarial expressions *)
+(** * Overview *)
 (**
-	An _adversarial expression_ contains no assertions and only
-	low locations. (We reserve assertions for verified code.)
+	There are at least two ways to prove robust safety.
+
+	My original statement of robust safety said roughly that if
+	context `c` satisfies a syntactic criterion and expression `e`
+	inhabits a semantic model, then `c[e]` inhabits the model. The
+	proof went as follows. First, prove the fundamental theorem of
+	logical relations (FTLR) saying that, for every expression `e`
+	in the language, if `e` satisfies a syntactic criterion, it
+	inhabits the model. The proof is by induction on `e`. Second,
+	use the FTLR to prove the *fundamental theorem of robust
+	safety* (FTRS) saying that, for every context `c`, if `c`
+	satisfies a syntactic criterion, it inhabits the model. The
+	proof is by induction on `c`, using the FTLR to deal with the
+	context's subexpressions. Finally, derive robust safety as a
+	trivial corollary of FTRS.
+
+	While straightforward, this original proof was not entirely
+	satisfying. The problem is that you end up reasoning about
+	every construct in the language *twice*, first when proving
+	the FTLR and second when proving the FTRS.
+
+	When I mentioned this annoyance to Deepak Garg, he suggested
+	switching to multi-holed contexts in order to dispense with
+	the FTLR and prove the FTRS directly. He guessed that
+	everything would work out and the FTLR---should you want
+	it---would be a simple corollary of the FTRS.
+
+	In the following, we apply Deepak's proof technique. The most
+	important property of the proof is that we reason about each
+	construct in the language exactly once. While this may not
+	seem a big deal for our simple heap language, it is
+	potentially a huge win for larger or more complicated
+	languages. Another benefit is that the resulting robust safety
+	theorem is more general, in that you can plug a context with a
+	list of expressions rather than a single expression. It says,
+	roughly, that if `c` satisfies a syntactic criterion and
+	`e_1`, …, `e_n` inhabit a semantic model, then `c[e_1, …,
+	e_n]` inhabits the model.
+**)
+
+(** * Contexts *)
+(**
+	The syntax of contexts is entirely standard, extending the
+	syntax of expressions with a constructor [CHole] for holes.
 *)
+Inductive ctx :=
+| CHole
+| CVar (x : string)
+| CRec (f : binder) (x : binder) (c : ctx)
+| CApp (c1 c2 : ctx)
+| CLit (lit : base_lit)
+| CUnOp (op : un_op) (c : ctx)
+| CBinOp (op : bin_op) (c1 c2 : ctx)
+| CIf (c0 c1 c2 : ctx)
+| CUnit
+| CPair (c1 c2 : ctx)
+| CFst (c : ctx)
+| CSnd (c : ctx)
+| CInjL (c : ctx)
+| CInjR (c : ctx)
+| CCase (c0 c1 c2 : ctx)
+| CAssert (c : ctx)
+| CFork (c : ctx)
+| CLoc (l : loc)
+| CAlloc (c : ctx)
+| CLoad (c : ctx)
+| CStore (c1 c2 : ctx)
+| CCAS (c0 c1 c2 : ctx).
 
-Class Adversarial Σ (A : Type) := Adv {
-  adv : A → iProp Σ;
-  adv_timeless a :> TimelessP (adv a);
-  adv_persistent a :> PersistentP (adv a);
-  adv_ne n :> Proper ((=) ==> dist n) adv
-}.
-Arguments Adv {_ _} _ _ _ _.
-Arguments adv {_ _ _} _ : simpl never.
-Instance: Params (@adv) 3.
+(** Embedding expressions [expr] in contexts [ctx]. *)
+Definition ctx_to_expr : ctx → option expr :=
+  fix go c :=
+  match c with
+  | CHole => None
+  | CVar x => Some (Var x)
+  | CRec f x c => e ← go c; Some (Rec f x e)
+  | CApp c1 c2 => e1 ← go c1; e2 ← go c2; Some (App e1 e2)
+  | CLit lit => Some (Lit lit)
+  | CUnOp op c => e ← go c; Some (UnOp op e)
+  | CBinOp op c1 c2 => e1 ← go c1; e2 ← go c2; Some (BinOp op e1 e2)
+  | CIf c0 c1 c2 => e0 ← go c0; e1 ← go c1; e2 ← go c2; Some (If e0 e1 e2)
+  | CUnit => Some Unit
+  | CPair c1 c2 => e1 ← go c1; e2 ← go c2; Some (Pair e1 e2)
+  | CFst c => e ← go c; Some (Fst e)
+  | CSnd c => e ← go c; Some (Snd e)
+  | CInjL c => e ← go c; Some (InjL e)
+  | CInjR c => e ← go c; Some (InjR e)
+  | CCase c0 c1 c2 => e0 ← go c0; e1 ← go c1; e2 ← go c2; Some (Case e0 e1 e2)
+  | CAssert c => e ← go c; Some (Assert e)
+  | CFork c => e ← go c; Some (Fork e)
+  | CLoc l => Some (Loc l)
+  | CAlloc c => e ← go c; Some (Alloc e)
+  | CLoad c => e ← go c; Some (Load e)
+  | CStore c1 c2 => e1 ← go c1; e2 ← go c2; Some (Store e1 e2)
+  | CCAS c0 c1 c2 => e0 ← go c0; e1 ← go c1; e2 ← go c2; Some (CAS e0 e1 e2)
+  end.
+Definition ctx_of_expr : expr → ctx :=
+  fix go e :=
+  match e with
+  | Var x => CVar x
+  | Rec f x e => CRec f x (go e)
+  | App e1 e2 => CApp (go e1) (go e2)
+  | Lit lit => CLit lit
+  | UnOp op e => CUnOp op (go e)
+  | BinOp op e1 e2 => CBinOp op (go e1) (go e2)
+  | If e0 e1 e2 => CIf (go e0) (go e1) (go e2)
+  | Unit => CUnit
+  | Pair e1 e2 => CPair (go e1) (go e2)
+  | Fst e => CFst (go e)
+  | Snd e => CSnd (go e)
+  | InjL e => CInjL (go e)
+  | InjR e => CInjR (go e)
+  | Case e0 e1 e2 => CCase (go e0) (go e1) (go e2)
+  | Assert e => CAssert (go e)
+  | Fork e => CFork (go e)
+  | Loc l => CLoc l
+  | Alloc e => CAlloc (go e)
+  | Load e => CLoad (go e)
+  | Store e1 e2 => CStore (go e1) (go e2)
+  | CAS e0 e1 e2 => CCAS (go e0) (go e1) (go e2)
+  end.
 
-Instance adv_proper `{Adversarial Σ A} : Proper ((=) ==> (≡)) adv.
-Proof. solve_proper. Qed.
+Instance ctx_of_expr_inj : Inj (=) (=) ctx_of_expr.
+Proof.
+  intros e1. induction e1=>e2 ?; simplify_eq/=; destruct e2;
+    simplify_eq/=; auto with f_equal.
+Qed.
+Lemma to_of_expr e : ctx_to_expr (ctx_of_expr e) = Some e.
+Proof. by induction e; simplify_option_eq; repeat f_equal. Qed.
+Lemma of_to_expr c e : ctx_to_expr c = Some e → ctx_of_expr e = c.
+Proof.
+  revert e. induction c; intros e ?; simplify_option_eq; auto with f_equal.
+Qed.
 
-Section adv_expr.
+(** * Multi-holed context plugging *)
+(**
+	Our multi-holed plugging operation plugs each hole, in turn,
+	with the next expression from a list of plugees, using the
+	dummy expression [Unit] when the list is exhausted and
+	ignoring unneeded plugees.
+*)
+Definition plugM (A : Type) : Type := list expr → A * list expr.
+Instance plugM_ret : MRet plugM := λ A x es, (x, es).
+Instance plugM_bind : MBind plugM := λ A B f mx es,
+  let p := mx es in f (p.1) (p.2).
+Definition next_plugee : plugM expr := λ es,
+  if es is e :: es then (e, es) else (Unit, []).	(* dummy *)
+Definition ctx_plugM : ctx → plugM expr :=
+  fix go c {struct c} :=
+  let unary := λ f c, e ← go c; mret (f e) in
+  let binary := λ f c1 c2, e1 ← go c1; unary (f e1) c2 in
+  let ternary := λ f c0 c1 c2, e0 ← go c0; binary (f e0) c1 c2 in
+  match c with
+  | CHole => next_plugee
+  | CVar x => mret (Var x)
+  | CRec f x c => unary (Rec f x) c
+  | CApp c1 c2 => binary App c1 c2
+  | CLit lit => mret (Lit lit)
+  | CUnOp op c => unary (UnOp op) c
+  | CBinOp op c1 c2 => binary (BinOp op) c1 c2
+  | CIf c0 c1 c2 => ternary If c0 c1 c2
+  | CUnit => mret Unit
+  | CPair c1 c2 => binary Pair c1 c2
+  | CFst c => unary Fst c
+  | CSnd c => unary Snd c
+  | CInjL c => unary InjL c
+  | CInjR c => unary InjR c
+  | CCase c0 c1 c2 => ternary Case c0 c1 c2
+  | CAssert c => unary Assert c
+  | CFork c => unary Fork c
+  | CLoc l => mret (Loc l)
+  | CAlloc c => unary Alloc c
+  | CLoad c => unary Load c
+  | CStore c1 c2 => binary Store c1 c2
+  | CCAS c0 c1 c2 => ternary CAS c0 c1 c2
+  end.
+Definition ctx_plug : ctx → list expr → expr := λ c es,
+  (ctx_plugM c es).1.
+Arguments ctx_plugM !_ _ / : assert.
+Arguments ctx_plug !_ _ / : assert.
+
+(** These tactics are probably overkill. *)
+Local Tactic Notation "simpl_plug" :=
+  repeat match goal with
+  | H : context [mret (M:=plugM) ?x ?es] |- _ =>
+    change (mret (M:=plugM) x es) with (x, es) in H
+  | H : context [mbind (M:=plugM) ?f ?mx ?es] |- _ =>
+    unfold mbind, plugM_bind in H
+  | H1 : ctx_plugM ?c ?es = (_, _), H2 : context[ctx_plugM ?c ?es] |- _ =>
+    rewrite H1 in H2
+  | H : ctx_plugM ?c ?es = (_, _) |- context[ctx_plugM ?c ?es] =>
+    idtac es; rewrite H
+  end.
+Local Tactic Notation "simplify_plug_eq" :=
+  repeat match goal with
+  | _ => progress simplify_eq/=
+  | _ => progress simpl_plug
+  end.
+Local Tactic Notation "destruct_plug" "as" simple_intropattern(IP) :=
+  match goal with
+  | |- context[(ctx_plugM ?c ?es).1] =>
+    destruct (ctx_plugM c es) as IP eqn:?; simplify_plug_eq
+  end.
+
+(** * Adversarial contexts *)
+(**
+	An _adversarial context_ contains no assertions and only low
+	locations. (This is a syntactic criterion.)
+*)
+Section adv_ctx.
   Context `{heapG Σ}.
 
-  Definition advexpr : expr → iProp Σ :=
-    fix rec e := match e with
-    | Var _ | Lit _ | Unit => True
-    | Assert _ => False
-    | Loc l => low l
-    | Rec _ _ e | UnOp _ e | Fst e | Snd e | InjL e | InjR e
-    | Fork e | Alloc e | Load e
-      => rec e
-    | App e1 e2 | BinOp _ e1 e2 | Pair e1 e2 | Store e1 e2 => rec e1 ∗ rec e2
-    | If e1 e2 e3 | Case e1 e2 e3 | CAS e1 e2 e3
-      => rec e1 ∗ rec e2 ∗ rec e3
+  Fixpoint adv_ctx (c : ctx) : iProp Σ :=
+    match c with
+    | CHole | CVar _ | CLit _ | CUnit => True
+    | CAssert _ => False
+    | CLoc l => low l
+    | CRec _ _ c | CUnOp _ c | CFst c | CSnd c | CInjL c | CInjR c
+    | CFork c | CAlloc c | CLoad c
+      => adv_ctx c
+    | CApp c1 c2 | CBinOp _ c1 c2 | CPair c1 c2 | CStore c1 c2
+      => adv_ctx c1 ∗ adv_ctx c2
+    | CIf c1 c2 c3 | CCase c1 c2 c3 | CCAS c1 c2 c3
+      => adv_ctx c1 ∗ adv_ctx c2 ∗ adv_ctx c3
     end%I.
-  Global Instance advexpr_persistent e : PersistentP (advexpr e).
-  Proof. elim: e=>//; by apply _. Qed.
-  Global Instance advexpr_timeless (e : expr) : TimelessP (advexpr e).
-  Proof. elim: e=>//; by apply _. Qed.
-  Global Instance advexpr_adv : Adversarial Σ expr := Adv advexpr _ _ _.
+  Global Instance adv_ctx_timeless c : TimelessP (adv_ctx c).
+  Proof. by elim: c=>//; apply _. Qed.
+  Global Instance adv_ctx_persistent c : PersistentP (adv_ctx c).
+  Proof. by elim: c=>//; apply _. Qed.
+  Global Instance adv_ctx_ne : Proper ((=) ==> dist n) adv_ctx.
+  Proof. apply _. Qed.
+  Global Instance adv_ctx_proper : Proper ((=) ==> (≡)) adv_ctx.
+  Proof. solve_proper. Qed.
+End adv_ctx.
+Typeclasses Opaque adv_ctx.
 
-  Lemma adv_expr e :
-    adv e ⊣⊢
-    match e with
-    | Var _ | Lit _ | Unit => True
-    | Assert _ => False
-    | Loc l => low l
-    | Rec _ _ e | UnOp _ e | Fst e | Snd e | InjL e | InjR e
-    | Fork e | Alloc e | Load e
-      => adv e
-    | App e1 e2 | BinOp _ e1 e2 | Pair e1 e2 | Store e1 e2 => adv e1 ∗ adv e2
-    | If e1 e2 e3 | Case e1 e2 e3 | CAS e1 e2 e3
-      => adv e1 ∗ adv e2 ∗ adv e3
-    end.
-  Proof. by case: e. Qed.
-End adv_expr.
-Typeclasses Opaque advexpr.
-
-(** * The fundamental theorem of logical relations *)
+(** * Meta-level adversaries *)
 (**
-	We model adversarial values and expressions with [low v] and
-	[WP e ?{{ low }}], respectively (see [low_val]). Our aim is to
-	show that, under the heap invariant, all adversarial
-	expressions inhabit the model.
+	To state the [robust_safety] theorem, we define a special case
+	of adversarial contexts at the meta-level. A *(meta-level)
+	adversary* is a context containing neither locations nor
+	assertions.
+*)
+Fixpoint AdvCtx (c : ctx) : Prop :=
+  match c with
+  | CHole | CVar _ | CLit _ | CUnit => True
+  | CAssert _ | CLoc _ => False
+  | CRec _ _ c | CUnOp _ c | CFst c | CSnd c | CInjL c | CInjR c
+  | CFork c | CAlloc c | CLoad c
+    => AdvCtx c
+  | CApp c1 c2 | CBinOp _ c1 c2 | CPair c1 c2 | CStore c1 c2
+    => AdvCtx c1 ∧ AdvCtx c2
+  | CIf c0 c1 c2 | CCase c0 c1 c2 | CCAS c0 c1 c2
+    => AdvCtx c0 ∧ AdvCtx c1 ∧ AdvCtx c2
+  end.
 
-	The proof is by induction on expressions. For the induction to
-	go through, we must generalize to account for substitution of
-	low values for variables. (Since the expression relation does
-	not imply progress, these need not be closing substitutions.)
- *)
-Section ftlr.
+Lemma adv_ctx_intro `{heapG Σ} c : AdvCtx c → adv_ctx c.
+Proof.
+  rewrite/uPred_valid. elim: c=>//=; intros;
+    repeat match goal with
+    | H : AdvCtx _ ∧ _ |- _ => destruct H
+    | IH : ?p → _, H : ?p |- _ => specialize (IH H); clear H
+    | IH : True ⊢ adv_ctx ?c |- True ⊢ adv_ctx ?c ∗ _ =>
+      rewrite -IH left_id; clear IH
+    | H : ?p |- ?p => exact H
+    end.
+Qed.
+
+(** * Robust safety *)
+(**
+	Our aim is to show that, under the heap invariant, if we plug
+	a bunch of semantically low expressions (i.e., code verified
+	to return a low value) into an adversarial context, the
+	resulting expression is semantically low.
+
+	The proof is by induction on contexts.
+*)
+Section robust_safety.
   Context `{heapG Σ}.
   Implicit Types γ : env.
+  Implicit Types c : ctx.
   Implicit Types e : expr.
   Implicit Types v : val.
 
+  (** Low environments send all binders to low values. *)
   Global Instance env_low : LowIntegrity Σ env :=
     Low (λ γ, [∗ map] v ∈ γ, low v)%I _ _.
-
-  Definition confined : expr → iProp Σ := λ e, (
-    ∀ γ, heap_ctx -∗ low γ -∗ adv e -∗ WP γ e ?{{ low }}
-  )%I.
-
   Lemma low_env γ : low γ ⊣⊢ [∗ map] v ∈ γ, low v. Proof. by []. Qed.
 
   Lemma low_env_empty : low (∅ : env) ⊣⊢ True.
   Proof. exact: big_sepM_empty. Qed.
-
   Lemma low_env_insert γ x v :
     γ !! x = None → low v -∗ low γ -∗ low (<[x:=v]>γ).
   Proof.
     do 2!rewrite low_env. move=>?. rewrite big_sepM_insert //.
     iIntros. by iFrame "#".
   Qed.
-
   Lemma low_env_singleton x v : low ({[x:=v]} : env) ⊣⊢ low v.
   Proof. exact: big_sepM_singleton. Qed.
-
   Lemma low_env_lookup γ x v : γ !! x = Some v → low γ -∗ low v.
   Proof. exact: big_sepM_lookup. Qed.
-
   Lemma low_env_delete γ x  : low γ -∗ low (delete x γ).
   Proof.
     rewrite low_env. apply big_sepM_mono. exact: delete_subseteq. done.
   Qed.
 
-  Lemma confined_var x : confined (Var x).
-  Proof.
-    iIntros (γ) "_ #Hγ _". rewrite substitute_expr.
-    case Hdom: (_ !! _)=>[v|]/=; last by iApply wp_stuck_var.
-    iApply wp_value'. by iApply (low_env_lookup with "[$Hγ]").
-  Qed.
-  Hint Extern 1 (_ ⊢ confined (Var _)) => rewrite -confined_var.
+  (**
+	An expression is *semantically low* if it is verified (under
+	the heap invariant) to either get stuck or return a low value.
 
-  Lemma confined_rec f x e : □ confined e -∗ confined (Rec f x e).
+	To deal with binders inductively, we generalize using a
+	substitution [γ] sending binders to low values. In contrast to
+	most work on logical relations, [γ] need not be a closing
+	substitution (because we permit a low expression to get
+	stuck).
+
+	The always modality makes [low_expr] persistent, which we need
+	in the proof that function contexts [CRec f x c] are
+	compatibile.
+  *)
+  Definition low_expr : expr → iProp Σ := λ e, (
+    □ ∀ γ, heap_ctx -∗ low γ -∗ WP γ e ?{{ low }}
+  )%I.
+
+  (**
+	As an important special case of low expressions, we say that
+	an expression is *verified code* if it is closed and verified
+	(under the heap invariant) to always returns a low value.
+
+	This is the notion of verified code used in the
+	[robust_safety] theorem.
+  *)
+  Definition verified_code : expr → iProp Σ := λ e, (
+    □ ∃ p, ⌜Closed [] e⌝ ∗ (heap_ctx -∗ WP e @ p; ⊤ {{ low }})
+  )%I.
+  (** Verified code satisfies [low_expr] (because it is closed). *)
+  Lemma verified_low e : verified_code e -∗ low_expr e.
   Proof.
-    iIntros "#IHe". iIntros (γ) "#Hh #Hγ #He".
-    rewrite adv_expr substitute_expr. set erec := substitute _ _.
+    iDestruct 1 as (p) "#[% He]".
+    iIntros "!#". iIntros (γ) "Hh _". rewrite substitute_closed.
+    rewrite -(wp_forget_progress p). iApply ("He" with "Hh").
+  Qed.
+
+  (**
+	A context is *semantically low* if, when plugged with low
+	expressions, it produces a low expression.
+  *)
+  Definition low_ctx : ctx → iProp Σ := λ c, (
+    ∀ es, ([∗ list] e ∈ es, low_expr e) -∗ low_expr (ctx_plug c es)
+  )%I.
+
+  (**
+	A context is *compatible* (with the logical relation
+	underlying low values) if, when it is adversarial, it is also
+	low. Compatibility lifts the syntactic [adv_ctx] to the
+	semantic [low_ctx].
+  *)
+  Definition compatible_ctx : ctx → iProp Σ := λ c, (
+    adv_ctx c -∗ low_ctx c
+  )%I.
+
+  (**
+	For our induction on contexts to go through, we strengthen
+	[low_ctx] and [compatible_ctx] to speak in terms of the
+	[ctx_plugM] operation and its state [es : list expr].
+  *)
+  Definition low_ctxM : ctx → iProp Σ := λ c, (
+    ∀ es e' es', ⌜ctx_plugM c es = (e', es')⌝ -∗
+    ([∗ list] e ∈ es, low_expr e) -∗
+    low_expr e' ∗ ([∗ list] e ∈ es', low_expr e)
+  )%I.
+  Definition compatible_ctxM : ctx → iProp Σ := λ c, (
+    adv_ctx c -∗ low_ctxM c
+  )%I.
+  Lemma compatible_ctx_intro c : compatible_ctxM c -∗ compatible_ctx c.
+  Proof.
+    iIntros "Hc Hadv". iIntros (es) "Hes".
+    iSpecialize ("Hc" with "Hadv"). rewrite/ctx_plug. destruct_plug as [e' es'].
+    iSpecialize ("Hc" $! es e' es' with "[%] Hes"); first done.
+    by iDestruct "Hc" as "[$ _]".
+  Qed.
+
+  (**
+	We use the following characterization of [compatible_ctxM] as
+	it's easier to work under the Iris proof mode.
+  *)
+  Definition compatible : ctx → iProp Σ := λ c, (
+    ∀ es e' es', ⌜ctx_plugM c es = (e', es')⌝ -∗ adv_ctx c -∗
+    ([∗ list] e ∈ es, low_expr e) -∗
+    low_expr e' ∗ ([∗ list] e ∈ es', low_expr e)
+  )%I.
+  Lemma compatible_spec c : compatible c ⊣⊢ compatible_ctxM c.
+  Proof.
+    apply equiv_spec; split.
+    - iIntros "Hc Hadv". iIntros (es e' es' ?) "Hes".
+      by iApply ("Hc" $! es e' es' with "[%] Hadv Hes").
+    - iIntros "Hc". iIntros (es e' es' ?) "Hadv Hes".
+      iSpecialize ("Hc" with "Hadv").
+      by iApply ("Hc" $! es e' es' with "[%] Hes").
+  Qed.
+
+  (**
+	For non-hole contexts, we need some boilerplate reasoning
+	about the context plugging operation to reduce compatibility
+	for contexts to a relation between low expressions.
+
+	The following three lemmas implement that boilerplate. (Coq
+	solves the complicated-looking side-conditions automatically.)
+  *)
+  Lemma compatible_nullary e c :
+    ctx_plugM c = mret e → low_expr e → compatible c.
+  Proof.
+    iIntros (Hnullary Hlow). iIntros (es e' es' Hplug) "_ Hes".
+    rewrite Hnullary{Hnullary} in Hplug. simplify_plug_eq. iFrame "Hes".
+    by rewrite -Hlow.
+  Qed.
+
+  Lemma compatible_unary (f : expr → expr) (g : ctx → ctx) c :
+    ctx_plugM (g c) = e ← ctx_plugM c; mret (f e) →
+    (adv_ctx (g c) -∗ adv_ctx c) →
+    (∀ e, low_expr e -∗ low_expr (f e)) →
+    compatible c -∗ compatible (g c).
+  Proof.
+    iIntros (Hunary Hadv Hlow) "IHc". iIntros (es e' es' Hplug) "Hadv Hes".
+    rewrite Hadv{Hadv}. rewrite Hunary{Hunary} in Hplug. simplify_plug_eq.
+    destruct_plug as [e es1].
+    iDestruct ("IHc" $! _ _ _ with "[%] Hadv Hes") as "[He $]"; first done.
+    iApply (Hlow with "He").
+  Qed.
+
+  Lemma compatible_binary (f : expr → expr → expr) (g : ctx → ctx → ctx) c1 c2 :
+    ctx_plugM (g c1 c2) = e1 ← ctx_plugM c1; e2 ← ctx_plugM c2; mret (f e1 e2) →
+    (adv_ctx (g c1 c2) -∗ adv_ctx c1 ∗ adv_ctx c2) →
+    (∀ e1 e2, low_expr e1 -∗ low_expr e2 -∗ low_expr (f e1 e2)) →
+    compatible c1 ∗ compatible c2 -∗ compatible (g c1 c2).
+  Proof.
+    iIntros (Hbinary Hadv Hlow) "[IHc1 IHc2]". iIntros (es e' es' Hplug).
+    rewrite Hadv{Hadv}. iIntros "[Hadv1 Hadv2] Hes".
+    rewrite Hbinary{Hbinary} in Hplug. simplify_plug_eq.
+    destruct_plug as [e1 es1].
+    iDestruct ("IHc1" $! _ _ _ with "[%] Hadv1 Hes") as "[He1 Hes]"; first done.
+    destruct_plug as [e2 es2].
+    iDestruct ("IHc2" $! _ _ _ with "[%] Hadv2 Hes") as "[He2 $]"; first done.
+    iApply (Hlow with "He1 He2").
+  Qed.
+
+  Lemma compatible_ternary (f : expr → expr → expr → expr)
+      (g : ctx → ctx → ctx → ctx) c0 c1 c2 :
+    ctx_plugM (g c0 c1 c2) =
+      e0 ← ctx_plugM c0; e1 ← ctx_plugM c1; e2 ← ctx_plugM c2;
+      mret (f e0 e1 e2) →
+    (adv_ctx (g c0 c1 c2) -∗ adv_ctx c0 ∗ adv_ctx c1 ∗ adv_ctx c2) →
+    (∀ e0 e1 e2, low_expr e0 -∗ low_expr e1 -∗ low_expr e2 -∗
+     low_expr (f e0 e1 e2)) →
+    compatible c0 ∗ compatible c1 ∗ compatible c2 -∗
+    compatible (g c0 c1 c2).
+  Proof.
+    iIntros (Hternary Hadv Hlow) "(IHc0&IHc1&IHc2)". iIntros (es e' es' Hplug).
+    rewrite Hadv{Hadv}. iIntros "(Hadv0&Hadv1&Hadv2) Hes".
+    rewrite Hternary{Hternary} in Hplug. simplify_plug_eq.
+    destruct_plug as [e0 es0].
+    iDestruct ("IHc0" $! _ _ _ with "[%] Hadv0 Hes") as "[He0 Hes]"; first done.
+    destruct_plug as [e1 es1].
+    iDestruct ("IHc1" $! _ _ _ with "[%] Hadv1 Hes") as "[He1 Hes]"; first done.
+    destruct_plug as [e2 es2].
+    iDestruct ("IHc2" $! _ _ _ with "[%] Hadv2 Hes") as "[He2 $]"; first done.
+    iApply (Hlow with "He0 He1 He2").
+  Qed.
+
+  (**
+	[Unit] is special because we need the fact that it's
+	semantically low twice. Once when showing [CHole] compatible
+	(because unit is the dummy expression used when there are no
+	plugees), and once when showing that [CUnit] is compatible.
+  *)
+  Lemma low_expr_Unit : True ⊢ low_expr Unit.
+  Proof.
+    iIntros "!#". iIntros (γ) "_ _". rewrite substitute_expr.
+    iApply wp_value; first done. by rewrite low_val.
+  Qed.
+
+  Lemma compatible_CHole : True ⊢ compatible CHole.
+  Proof.
+    iIntros (es e' es' ?) "_ Hes". destruct es as [|e es]; simplify_plug_eq.
+    - iFrame "Hes". by rewrite -low_expr_Unit.
+    - by rewrite big_sepL_cons.
+  Qed.
+  Hint Extern 1 (_ ⊢ compatible CHole) => rewrite -compatible_CHole.
+
+  Lemma compatible_CVar x : True ⊢ compatible (CVar x).
+  Proof.
+    rewrite compatible_nullary=>//.
+    iIntros "!#". iIntros (γ) "_ Hγ". rewrite substitute_expr.
+    case Hdom: (_ !! _)=>[v|]/=; last by iApply wp_stuck_var.
+    iApply wp_value'. by iApply (low_env_lookup with "Hγ").
+  Qed.
+  Hint Extern 1 (_ ⊢ compatible (CVar _)) => rewrite -compatible_CVar.
+
+  Lemma compatible_CRec f x c : compatible c -∗ compatible (CRec f x c).
+  Proof.
+    rewrite compatible_unary=>//{c}e.
+    iIntros "#IHe !#". iIntros (γ) "#Hh #Hγ". rewrite substitute_expr.
+    set erec := substitute _ _.
     case: (decide (Closed (f :b: x :b: []) erec)) => ?;
       last by iApply wp_stuck_rec_open.
     iApply wp_value; first exact: to_val_rec.
@@ -133,887 +521,331 @@ Section ftlr.
     iIntros (v2) "#Hv2". case: (decide (x = f))=>?.
     { subst. rewrite -> subst_subst'; last done.	(* ssr rewrite fails *)
       rewrite of_val_rec subst_substitute; first by rewrite lookup_delete.
-      iApply ("IHe" with "Hh [] He").
+      iApply ("IHe" with "Hh []").
       rewrite insert_delete. iApply (low_env_insert with "Hvrec");
         first by rewrite lookup_delete.
       by iApply (low_env_delete with "Hγ"). }
     rewrite of_val_rec subst_substitute; first by rewrite lookup_delete.
     rewrite subst_substitute; first by rewrite
       lookup_insert_ne // lookup_delete_ne // lookup_delete.
-    iApply ("IHe" with "Hh [] He").
+    iApply ("IHe" with "Hh []").
     iApply (low_env_insert with "Hv2"); first by rewrite
       lookup_insert_ne // lookup_delete_ne // lookup_delete.
     iApply (low_env_insert with "Hvrec"); first by rewrite
       lookup_delete.
     do 2!iApply low_env_delete. iExact "Hγ".
   Qed.
-  Hint Extern 1 (_ ⊢ confined (Rec _ _ _))
-    => rewrite -confined_rec; exact: always_intro.
+  Hint Extern 1 (_ ⊢ compatible (CRec _ _ _)) => rewrite -compatible_CRec.
 
-  Lemma confined_app e1 e2 : confined e1 ∗ confined e2 -∗ confined (App e1 e2).
+  Lemma compatible_CApp c1 c2 :
+    compatible c1 ∗ compatible c2 -∗ compatible (CApp c1 c2).
   Proof.
-    iIntros "[IHe1 IHe2]". iIntros (γ) "#Hh #Hγ Happ".
-    rewrite adv_expr substitute_expr. iDestruct "Happ" as "(He1&He2)".
-    iApply (wp_on_val_app_bind with "[IHe1 He1]").
-    - by iApply ("IHe1" with "Hh Hγ He1").
-    - by iApply ("IHe2" with "Hh Hγ He2").
+    rewrite compatible_binary=>//{c1 c2}e1 e2.
+    iIntros "#IHe1 #IHe2 !#". iIntros (γ) "#Hh #Hγ". rewrite substitute_expr.
+    iApply (wp_on_val_app_bind with "[]").
+    - by iApply ("IHe1" with "Hh Hγ").
+    - by iApply ("IHe2" with "Hh Hγ").
   Qed.
-  Hint Extern 1 (_ ⊢ confined (App _ _)) => rewrite -confined_app.
+  Hint Extern 1 (_ ⊢ compatible (CApp _ _)) => rewrite -compatible_CApp.
 
-  Lemma confined_lit lit : confined (Lit lit).
+  Lemma compatible_CLit lit : True ⊢ compatible (CLit lit).
   Proof.
-    iIntros (γ) "_ _ _". rewrite substitute_expr.
+    rewrite compatible_nullary=>//.
+    iIntros "!#". iIntros (γ) "_ _". rewrite substitute_expr.
     iApply wp_value; first done. by rewrite low_val.
   Qed.
-  Hint Extern 1 (_ ⊢ confined (Lit _)) => rewrite -confined_lit.
+  Hint Extern 1 (_ ⊢ compatible (CLit _)) => rewrite -compatible_CLit.
 
-  Lemma confined_un_op op e : confined e -∗ confined (UnOp op e).
+  Lemma compatible_CUnOp op c : compatible c -∗ compatible (CUnOp op c).
   Proof.
-    iIntros "IHe". iIntros (γ) "Hh Hγ He". rewrite adv_expr substitute_expr.
-    iApply wp_on_val_un_op_bind. by iApply ("IHe" with "Hh Hγ He").
+    rewrite compatible_unary=>//{c}e.
+    iIntros "#IHe !#". iIntros (γ) "Hh Hγ". rewrite substitute_expr.
+    iApply wp_on_val_un_op_bind. by iApply ("IHe" with "Hh Hγ").
   Qed.
-  Hint Extern 1 (_ ⊢ confined (UnOp _ _)) => rewrite -confined_un_op.
+  Hint Extern 1 (_ ⊢ compatible (CUnOp _ _)) => rewrite -compatible_CUnOp.
 
-  Lemma confined_bin_op op e1 e2 :
-    confined e1 ∗ confined e2 -∗ confined (BinOp op e1 e2).
+  Lemma compatible_CBinOp op c1 c2 :
+    compatible c1 ∗ compatible c2 -∗ compatible (CBinOp op c1 c2).
   Proof.
-    iIntros "[IHe1 IHe2]". iIntros (γ) "#Hh #Hγ Hop".
-    rewrite adv_expr substitute_expr. iDestruct "Hop" as "(He1&He2)".
-    iApply (wp_on_val_bin_op_bind with "[IHe1 He1]").
-    - by iApply ("IHe1" with "Hh Hγ He1").
-    - by iApply ("IHe2" with "Hh Hγ He2").
+    rewrite compatible_binary=>//{c1 c2}e1 e2.
+    iIntros "#IHe1 #IHe2 !#". iIntros (γ) "#Hh #Hγ". rewrite substitute_expr.
+    iApply (wp_on_val_bin_op_bind with "[IHe1]").
+    - by iApply ("IHe1" with "Hh Hγ").
+    - by iApply ("IHe2" with "Hh Hγ").
   Qed.
-  Hint Extern 1 (_ ⊢ confined (BinOp _ _ _)) => rewrite -confined_bin_op.
+  Hint Extern 1 (_ ⊢ compatible (CBinOp _ _ _)) => rewrite -compatible_CBinOp.
 
-  Lemma confined_if e e1 e2 :
-    confined e ∗ confined e1 ∗ confined e2 -∗ confined (If e e1 e2).
+  Lemma compatible_CIf c0 c1 c2 :
+    compatible c0 ∗ compatible c1 ∗ compatible c2 -∗ compatible (CIf c0 c1 c2).
   Proof.
-    iIntros "(IHe&IHe1&IHe2)". iIntros (γ) "#Hh #Hγ Hif".
-    rewrite adv_expr substitute_expr. iDestruct "Hif" as "(He&He1&He2)".
-    wp_apply (wp_any_if_bind with "[IHe He]"); last iSplit.
-    - by iApply ("IHe" with "Hh Hγ He").
-    - by iApply ("IHe1" with "Hh Hγ He1").
-    - by iApply ("IHe2" with "Hh Hγ He2").
+    rewrite compatible_ternary=>//{c0 c1 c2}e0 e1 e2.
+    iIntros "#IHe0 #IHe1 #IHe2 !#". iIntros (γ) "#Hh #Hγ".
+    rewrite substitute_expr. wp_apply (wp_any_if_bind with "[]"); last iSplit.
+    - by iApply ("IHe0" with "Hh Hγ").
+    - by iApply ("IHe1" with "Hh Hγ").
+    - by iApply ("IHe2" with "Hh Hγ").
   Qed.
-  Hint Extern 1 (_ ⊢ confined (If _ _ _)) => rewrite -confined_if.
+  Hint Extern 1 (_ ⊢ compatible (CIf _ _ _)) => rewrite -compatible_CIf.
 
-  Lemma confined_unit : confined Unit.
+  Lemma compatible_CUnit : True ⊢ compatible CUnit.
+  Proof. rewrite compatible_nullary//. exact: low_expr_Unit. Qed.
+  Hint Extern 1 (_ ⊢ compatible CUnit) => rewrite -compatible_CUnit.
+
+  Lemma compatible_CPair c1 c2 :
+    compatible c1 ∗ compatible c2 -∗ compatible (CPair c1 c2).
   Proof.
-    iIntros (γ) "_ _ _". rewrite substitute_expr.
-    iApply wp_value; first done. by rewrite low_val.
+    rewrite compatible_binary=>//{c1 c2}e1 e2.
+    iIntros "#IHe1 #IHe2 !#". iIntros (γ) "#Hh #Hγ".
+    rewrite substitute_expr. iApply (wp_on_val_pair_bind with "[]").
+    - by iApply ("IHe1" with "Hh Hγ").
+    - by iApply ("IHe2" with "Hh Hγ").
   Qed.
-  Hint Extern 1 (_ ⊢ confined Unit) => rewrite -confined_unit.
+  Hint Extern 1 (_ ⊢ compatible (CPair _ _)) => rewrite -compatible_CPair.
 
-  Lemma confined_pair e1 e2 :
-    confined e1 ∗ confined e2 -∗ confined (Pair e1 e2).
+  Lemma compatible_CFst c : compatible c -∗ compatible (CFst c).
   Proof.
-    iIntros "[IHe1 IHe2]". iIntros (γ) "#Hh #Hγ Hp".
-    rewrite adv_expr substitute_expr. iDestruct "Hp" as "(He1&He2)".
-    iApply (wp_on_val_pair_bind with "[IHe1 He1]").
-    - by iApply ("IHe1" with "Hh Hγ He1").
-    - by iApply ("IHe2" with "Hh Hγ He2").
+    rewrite compatible_unary=>//{c}e.
+    iIntros "#IHe !#". iIntros (γ) "Hh Hγ". rewrite substitute_expr.
+    iApply wp_on_val_fst_bind. by iApply ("IHe" with "Hh Hγ").
   Qed.
-  Hint Extern 1 (_ ⊢ confined (Pair _ _)) => rewrite -confined_pair.
+  Hint Extern 1 (_ ⊢ compatible (CFst _)) => rewrite -compatible_CFst.
 
-  Lemma confined_fst e : confined e -∗ confined (Fst e).
+  Lemma compatible_CSnd c : compatible c -∗ compatible (CSnd c).
   Proof.
-    iIntros "IHe". iIntros (γ) "Hh Hγ He". rewrite adv_expr substitute_expr.
-    iApply wp_on_val_fst_bind. by iApply ("IHe" with "Hh Hγ He").
+    rewrite compatible_unary=>//{c}e.
+    iIntros "#IHe !#". iIntros (γ) "Hh Hγ". rewrite substitute_expr.
+    iApply wp_on_val_snd_bind. by iApply ("IHe" with "Hh Hγ").
   Qed.
-  Hint Extern 1 (_ ⊢ confined (Fst _)) => rewrite -confined_fst.
+  Hint Extern 1 (_ ⊢ compatible (CSnd _)) => rewrite -compatible_CSnd.
 
-  Lemma confined_snd e : confined e -∗ confined (Snd e).
+  Lemma compatible_CInjL c : compatible c -∗ compatible (CInjL c).
   Proof.
-    iIntros "IHe". iIntros (γ) "Hh Hγ He". rewrite adv_expr substitute_expr.
-    iApply wp_on_val_snd_bind. by iApply ("IHe" with "Hh Hγ He").
+    rewrite compatible_unary=>//{c}e.
+    iIntros "#IHe !#". iIntros (γ) "Hh Hγ". rewrite substitute_expr.
+    iApply wp_on_val_inl_bind. by iApply ("IHe" with "Hh Hγ").
   Qed.
-  Hint Extern 1 (_ ⊢ confined (Snd _)) => rewrite -confined_snd.
+  Hint Extern 1 (_ ⊢ compatible (CInjL _)) => rewrite -compatible_CInjL.
 
-  Lemma confined_inl e : confined e -∗ confined (InjL e).
+  Lemma compatible_CInjR c : compatible c -∗ compatible (CInjR c).
   Proof.
-    iIntros "IHe". iIntros (γ) "Hh Hγ He". rewrite adv_expr substitute_expr.
-    iApply wp_on_val_inl_bind. by iApply ("IHe" with "Hh Hγ He").
+    rewrite compatible_unary=>//{c}e.
+    iIntros "#IHe !#". iIntros (γ) "Hh Hγ". rewrite substitute_expr.
+    iApply wp_on_val_inr_bind. by iApply ("IHe" with "Hh Hγ").
   Qed.
-  Hint Extern 1 (_ ⊢ confined (InjL _)) => rewrite -confined_inl.
+  Hint Extern 1 (_ ⊢ compatible (CInjR _)) => rewrite -compatible_CInjR.
 
-  Lemma confined_inr e : confined e -∗ confined (InjR e).
+  Lemma compatible_CCase c0 c1 c2 :
+    compatible c0 ∗ compatible c1 ∗ compatible c2 -∗
+    compatible (CCase c0 c1 c2).
   Proof.
-    iIntros "IHe". iIntros (γ) "Hh Hγ He". rewrite adv_expr substitute_expr.
-    iApply wp_on_val_inr_bind. by iApply ("IHe" with "Hh Hγ He").
-  Qed.
-  Hint Extern 1 (_ ⊢ confined (InjR _)) => rewrite -confined_inr.
-
-  Lemma confined_case e e1 e2 :
-    confined e ∗ confined e1 ∗ confined e2 -∗ confined (Case e e1 e2).
-  Proof.
-    iIntros "(IHe&IHe1&IHe2)". iIntros (γ) "#Hh #Hγ Hc".
-    rewrite adv_expr substitute_expr. iDestruct "Hc" as "(He&He1&He2)".
-    wp_apply (wp_on_val_case_bind with "[IHe He]"); last (iIntros (v) "Hv"; iSplit).
-    - by iApply ("IHe" with "Hh Hγ He").
+    rewrite compatible_ternary=>//{c0 c1 c2}e0 e1 e2.
+    iIntros "#IHe0 #IHe1 #IHe2 !#". iIntros (γ) "#Hh #Hγ".
+    rewrite substitute_expr.
+    wp_apply (wp_on_val_case_bind with "[]"); last (iIntros (v) "Hv"; iSplit).
+    - by iApply ("IHe0" with "Hh Hγ").
     - iApply (wp_on_val_app_bind with "[-Hv]").
-      by iApply ("IHe1" with "Hh Hγ He1"). by wp_value.
+      by iApply ("IHe1" with "Hh Hγ"). by wp_value.
     - iApply (wp_on_val_app_bind with "[-Hv]").
-      by iApply ("IHe2" with "Hh Hγ He2"). by wp_value.
+      by iApply ("IHe2" with "Hh Hγ"). by wp_value.
   Qed.
-  Hint Extern 1 (_ ⊢ confined (Case _ _ _)) => rewrite -confined_case.
+  Hint Extern 1 (_ ⊢ compatible (CCase _ _ _)) => rewrite -compatible_CCase.
 
-  Lemma confined_assert e : confined (Assert e).
-  Proof. iIntros (γ) "_ _ He". rewrite adv_expr. by iExFalso. Qed.
-  Hint Extern 1 (_ ⊢ confined (Assert _)) => rewrite -confined_assert.
+  (**
+	[CAssert] is special because it cannot occur in adversarial
+	contexts.
+  *)
+  Lemma compatible_CAssert c : True ⊢ compatible (CAssert c).
+  Proof. iIntros (es e' es' _) "/= Hadv". by iExFalso. Qed.
+  Hint Extern 1 (_ ⊢ compatible (CAssert _)) => rewrite -compatible_CAssert.
 
-  Lemma confined_fork e : confined e -∗ confined (Fork e).
+  Lemma compatible_CFork c : compatible c -∗ compatible (CFork c).
   Proof.
-    iIntros "IHe". iIntros (γ) "Hh Hγ He". rewrite adv_expr substitute_expr.
-    wp_apply wp_on_val_fork. by iApply ("IHe" with "Hh Hγ He").
+    rewrite compatible_unary=>//{c}e.
+    iIntros "#IHe !#". iIntros (γ) "Hh Hγ". rewrite substitute_expr.
+    wp_apply wp_on_val_fork. by iApply ("IHe" with "Hh Hγ").
   Qed.
-  Hint Extern 1 (_ ⊢ confined (Fork _)) => rewrite -confined_fork.
+  Hint Extern 1 (_ ⊢ compatible (CFork _)) => rewrite -compatible_CFork.
 
-  Lemma confined_loc l : confined (Loc l).
+  (**
+	[CLoc] is special because all locations in adversarial
+	contexts are low.
+  *)
+  Lemma compatible_CLoc l : True ⊢ compatible (CLoc l).
   Proof.
-    iIntros (γ) "_ _ ?". rewrite adv_expr substitute_expr.
+    iIntros (es e es' ?) "#Hadv Hes". simplify_plug_eq. iFrame "Hes".
+    iIntros "!#". iIntros (γ) "_ _". rewrite substitute_expr.
     iApply wp_value; first done. by rewrite low_val.
   Qed.
-  Hint Extern 1 (_ ⊢ confined (Loc _)) => rewrite -confined_loc.
+  Hint Extern 1 (_ ⊢ compatible (CLoc _)) => rewrite -compatible_CLoc.
 
-  Lemma confined_alloc e : confined e -∗ confined (Alloc e).
+  Lemma compatible_CAlloc c : compatible c -∗ compatible (CAlloc c).
   Proof.
-    iIntros "IHe". iIntros (γ) "#Hh Hγ He". rewrite adv_expr substitute_expr.
-    iApply (wp_low_alloc_bind with "Hh"). done. by iApply ("IHe" with "Hh Hγ He").
+    rewrite compatible_unary=>//{c}e.
+    iIntros "#IHe !#". iIntros (γ) "#Hh Hγ". rewrite substitute_expr.
+    iApply (wp_low_alloc_bind with "Hh"). done. by iApply ("IHe" with "Hh Hγ").
   Qed.
-  Hint Extern 1 (_ ⊢ confined (Alloc _)) => rewrite -confined_alloc.
+  Hint Extern 1 (_ ⊢ compatible (CAlloc _)) => rewrite -compatible_CAlloc.
 
-  Lemma confined_load e : confined e -∗ confined (Load e).
+  Lemma compatible_CLoad c : compatible c -∗ compatible (CLoad c).
   Proof.
-    iIntros "IHe". iIntros (γ) "#Hh Hγ He". rewrite adv_expr substitute_expr.
-    iApply (wp_low_load_bind with "Hh"). done. by iApply ("IHe" with "Hh Hγ He").
+    rewrite compatible_unary=>//{c}e.
+    iIntros "#IHe !#". iIntros (γ) "#Hh Hγ". rewrite substitute_expr.
+    iApply (wp_low_load_bind with "Hh"). done. by iApply ("IHe" with "Hh Hγ").
   Qed.
-  Hint Extern 1 (_ ⊢ confined (Load _)) => rewrite -confined_load.
+  Hint Extern 1 (_ ⊢ compatible (CLoad _)) => rewrite -compatible_CLoad.
 
-  Lemma confined_store e1 e2 :
-    confined e1 ∗ confined e2 -∗ confined (Store e1 e2).
+  Lemma compatible_CStore c1 c2 :
+    compatible c1 ∗ compatible c2 -∗ compatible (CStore c1 c2).
   Proof.
-    iIntros "[IHe1 IHe2]". iIntros (γ) "#Hh #Hγ Hstore".
-    rewrite adv_expr substitute_expr. iDestruct "Hstore" as "(He1&He2)".
-    iApply (wp_low_store_bind with "Hh [IHe1 He1]"); first done.
-    - by iApply ("IHe1" with "Hh Hγ He1").
-    - by iApply ("IHe2" with "Hh Hγ He2").
+    rewrite compatible_binary=>//{c1 c2}e1 e2.
+    iIntros "#IHe1 #IHe2 !#". iIntros (γ) "#Hh #Hγ". rewrite substitute_expr.
+    iApply (wp_low_store_bind with "Hh []"); first done.
+    - by iApply ("IHe1" with "Hh Hγ").
+    - by iApply ("IHe2" with "Hh Hγ").
   Qed.
-  Hint Extern 1 (_ ⊢ confined (Store _ _)) => rewrite -confined_store.
+  Hint Extern 1 (_ ⊢ compatible (CStore _ _)) => rewrite -compatible_CStore.
 
-  Lemma confined_cas e0 e1 e2 :
-    confined e0 ∗ confined e1 ∗ confined e2 -∗ confined (CAS e0 e1 e2).
+  Lemma compatible_CCAS c0 c1 c2 :
+    compatible c0 ∗ compatible c1 ∗ compatible c2 -∗
+    compatible (CCAS c0 c1 c2).
   Proof.
-    iIntros "(IHe0&IHe1&IHe2)". iIntros (γ) "#Hh #Hγ Hcas".
-    rewrite adv_expr substitute_expr. iDestruct "Hcas" as "(He0&He1&He2)".
-    iApply (wp_low_cas_bind with "Hh [IHe0 He0] [IHe1 He1]"); first done.
-    - by iApply ("IHe0" with "Hh Hγ He0").
-    - by iApply ("IHe1" with "Hh Hγ He1").
-    - by iApply ("IHe2" with "Hh Hγ He2").
+    rewrite compatible_ternary=>//{c0 c1 c2}e0 e1 e2.
+    iIntros "#IHe0 #IHe1 #IHe2 !#". iIntros (γ) "#Hh #Hγ". rewrite substitute_expr.
+    iApply (wp_low_cas_bind with "Hh [] []"); first done.
+    - by iApply ("IHe0" with "Hh Hγ").
+    - by iApply ("IHe1" with "Hh Hγ").
+    - by iApply ("IHe2" with "Hh Hγ").
   Qed.
-  Hint Extern 1 (_ ⊢ confined (CAS _ _ _)) => rewrite -confined_cas.
+  Hint Extern 1 (_ ⊢ compatible (CCAS _ _ _)) => rewrite -compatible_CCAS.
 
   Hint Extern 2 =>
     match goal with
-    | IH : True ⊢ confined ?e |- True ⊢ confined (_ ?e) => rewrite IH
+    | IH : True ⊢ compatible ?c |- True ⊢ compatible (_ ?c) => rewrite IH
     end.
   Hint Extern 2 =>
     match goal with
-    | IH1 : True ⊢ confined ?e1, IH2 : True ⊢ confined ?e2
-      |- True ⊢ confined (_ ?e1 ?e2)
+    | IH1 : True ⊢ compatible ?c1, IH2 : True ⊢ compatible ?c2
+      |- True ⊢ compatible (_ ?c1 ?c2)
       => rewrite (True_sep_1 True) {1}IH1 IH2
     end.
   Hint Extern 2 =>
     match goal with
-    | IH1 : True ⊢ confined ?e1, IH2 : True ⊢ confined ?e2,
-      IH3 : True ⊢ confined ?e3 |- True ⊢ confined (_ ?e1 ?e2 ?e3)
+    | IH1 : True ⊢ compatible ?c1, IH2 : True ⊢ compatible ?c2,
+      IH3 : True ⊢ compatible ?c3 |- True ⊢ compatible (_ ?c1 ?c2 ?c3)
       => rewrite (True_sep_1 True) {2}(True_sep_1 True) {1}IH1 {1}IH2 IH3
     end.
 
-  Theorem ftlr e : confined e.
-  Proof. rewrite/uPred_valid. by induction e; auto. Qed.
-
-  Corollary ftlr_alt γ e Φ :
-    heap_ctx ⊢ low γ -∗ adv e -∗ (∀ v, low v -∗ Φ v) -∗ WP γ e ?{{ Φ }}.
+  (**
+	The fundamental theorem of robust safety: all adversarial
+	contexts are semantically low.
+  *)
+  Theorem fundamental_theorem_robust_safety c : compatible_ctx c.
   Proof.
-    iIntros "Hh Hγ He". rewrite -wp_wand. by iApply (ftlr with "Hh Hγ He").
-  Qed.
-End ftlr.
-
-(** * Contexts *)
-(**
-	Contexts are expressions with a single hole. The following
-	definition must agree with [heap_lang.expr].
-*)
-Inductive ctx :=
-  | CHole
-  | CRec of binder & binder & ctx
-  | CAppL of ctx & expr
-  | CAppR of expr & ctx
-  | CUnOp of un_op & ctx
-  | CBinOpL of bin_op & ctx & expr
-  | CBinOpR of bin_op & expr & ctx
-  | CIf of ctx & expr & expr
-  | CIfL of expr & ctx & expr
-  | CIfR of expr & expr & ctx
-  | CPairL of ctx & expr
-  | CPairR of expr & ctx
-  | CFst of ctx
-  | CSnd of ctx
-  | CInjL of ctx
-  | CInjR of ctx
-  | CCase of ctx & expr & expr
-  | CCaseL of expr & ctx & expr
-  | CCaseR of expr & expr & ctx
-  | CAssert of ctx
-  | CFork of ctx
-  | CAlloc of ctx
-  | CLoad of ctx
-  | CStoreL of ctx & expr
-  | CStoreR of expr & ctx
-  | CCASL of ctx & expr & expr
-  | CCASM of expr & ctx & expr
-  | CCASR of expr & expr & ctx.
-
-Fixpoint ctx_fill (C : ctx) (e : expr) : expr :=
-  let rec := λ C, ctx_fill C e in
-  match C with
-  | CHole => e
-  | CRec f x C => Rec f x (rec C)
-  | CAppL C1 e2 => App (rec C1) e2
-  | CAppR e1 C2 => App e1 (rec C2)
-  | CUnOp op C => UnOp op (rec C)
-  | CBinOpL op C1 e2 => BinOp op (rec C1) e2
-  | CBinOpR op e1 C2 => BinOp op e1 (rec C2)
-  | CIf C0 e1 e2 => If (rec C0) e1 e2
-  | CIfL e0 C1 e2 => If e0 (rec C1) e2
-  | CIfR e0 e1 C2 => If e0 e1 (rec C2)
-  | CPairL C1 e2 => Pair (rec C1) e2
-  | CPairR e1 C2 => Pair e1 (rec C2)
-  | CFst C => Fst (rec C)
-  | CSnd C => Snd (rec C)
-  | CInjL C => InjL (rec C)
-  | CInjR C => InjR (rec C)
-  | CCase C0 e1 e2 => Case (rec C0) e1 e2
-  | CCaseL e0 C1 e2 => Case e0 (rec C1) e2
-  | CCaseR e0 e1 C2 => Case e0 e1 (rec C2)
-  | CAssert C => Assert (rec C)
-  | CFork C => Fork (rec C)
-  | CAlloc C => Alloc (rec C)
-  | CLoad C => Load (rec C)
-  | CStoreL C1 e2 => Store (rec C1) e2
-  | CStoreR e1 C2 => Store e1 (rec C2)
-  | CCASL C0 e1 e2 => CAS (rec C0) e1 e2
-  | CCASM e0 C1 e2 => CAS e0 (rec C1) e2
-  | CCASR e0 e1 C2 => CAS e0 e1 (rec C2)
-  end.
-
-(**
-	An _adversarial context_ contains no assertions and only
-	adversarial subexpressions.
-*)
-Section adv_ctx.
-  Context `{heapG Σ}.
-  Implicit Types C : ctx.
-
-  Definition advctx : ctx → iProp Σ :=
-    fix rec C := match C with
-    | CHole => True
-    | CAssert _ => False
-    | CRec _ _ C | CUnOp _ C | CFst C | CSnd C | CInjL C | CInjR C
-    | CFork C | CAlloc C | CLoad C
-      => rec C
-    | CAppL C1 e2 | CBinOpL _ C1 e2 | CPairL C1 e2 | CStoreL C1 e2
-      => rec C1 ∗ adv e2
-    | CAppR e1 C2 | CBinOpR _ e1 C2 | CPairR e1 C2 | CStoreR e1 C2
-      => adv e1 ∗ rec C2
-    | CIf C0 e1 e2 | CCase C0 e1 e2 | CCASL C0 e1 e2
-      => rec C0 ∗ adv e1 ∗ adv e2
-    | CIfL e0 C1 e2 | CCaseL e0 C1 e2 | CCASM e0 C1 e2
-      => adv e0 ∗ rec C1 ∗ adv e2
-    | CIfR e0 e1 C2 | CCaseR e0 e1 C2 | CCASR e0 e1 C2
-      => adv e0 ∗ adv e1 ∗ rec C2
-    end%I.
-  Global Instance advctx_persistent C : PersistentP (advctx C).
-  Proof. elim: C=>//; by apply _. Qed.
-  Global Instance advctx_timeless (C : ctx) : TimelessP (advctx C).
-  Proof. elim: C=>//; by apply _. Qed.
-  Global Instance advctx_adv : Adversarial Σ ctx := Adv advctx _ _ _.
-
-  Lemma adv_ctx C :
-    adv C ⊣⊢
-    match C with
-    | CHole => True
-    | CAssert _ => False
-    | CRec _ _ C | CUnOp _ C | CFst C | CSnd C | CInjL C | CInjR C
-    | CFork C | CAlloc C | CLoad C
-      => adv C
-    | CAppL C1 e2 | CBinOpL _ C1 e2 | CPairL C1 e2 | CStoreL C1 e2
-      => adv C1 ∗ adv e2
-    | CAppR e1 C2 | CBinOpR _ e1 C2 | CPairR e1 C2 | CStoreR e1 C2
-      => adv e1 ∗ adv C2
-    | CIf C0 e1 e2 | CCase C0 e1 e2 | CCASL C0 e1 e2
-      => adv C0 ∗ adv e1 ∗ adv e2
-    | CIfL e0 C1 e2 | CCaseL e0 C1 e2 | CCASM e0 C1 e2
-      => adv e0 ∗ adv C1 ∗ adv e2
-    | CIfR e0 e1 C2 | CCaseR e0 e1 C2 | CCASR e0 e1 C2
-      => adv e0 ∗ adv e1 ∗ adv C2
-    end%I.
-  Proof. by case: C. Qed.
-End adv_ctx.
-Typeclasses Opaque advctx.
-
-(** Sanity check. *)
-(**
-	To catch changes to [expr] that aren't reflected in [ctx], we
-	embed evaluation contexts in contexts and prove the filling
-	functions match up.
-*)
-Local Notation ectx := (list ectx_item).
-
-Definition of_ectx_item (Ki : ectx_item) (C : ctx) : ctx :=
-  match Ki with
-  | AppLCtx e2 => CAppL C e2
-  | AppRCtx v1 => CAppR (of_val v1) C
-  | UnOpCtx op => CUnOp op C
-  | BinOpLCtx op e2 => CBinOpL op C e2
-  | BinOpRCtx op v1 => CBinOpR op (of_val v1) C
-  | IfCtx e1 e2 => CIf C e1 e2
-  | PairLCtx e2 => CPairL C e2
-  | PairRCtx v1 => CPairR (of_val v1) C
-  | FstCtx => CFst C
-  | SndCtx => CSnd C
-  | InjLCtx => CInjL C
-  | InjRCtx => CInjR C
-  | CaseCtx e1 e2 => CCase C e1 e2
-  | AssertCtx => CAssert C
-  | AllocCtx => CAlloc C
-  | LoadCtx => CLoad C
-  | StoreLCtx e2 => CStoreL C e2
-  | StoreRCtx v1 => CStoreR (of_val v1) C
-  | CasLCtx e1 e2 => CCASL C e1 e2
-  | CasMCtx v0 e2 => CCASM (of_val v0) C e2
-  | CasRCtx v0 v1 => CCASR (of_val v0) (of_val v1) C
-  end.
-
-Definition of_ectx : ectx → ctx := foldr of_ectx_item CHole.
-
-Fixpoint to_ectx (C : ctx) : option ectx :=
-  let rec := λ C Ki, K ← to_ectx C; Some (Ki :: K) in
-  let recv := λ e C f, v ← to_val e; rec C $ f v in
-  match C with
-  | CHole => Some []
-  | CAppL C e2 => rec C $ AppLCtx e2
-  | CAppR e1 C => recv e1 C $ AppRCtx
-  | CUnOp op C => rec C $ UnOpCtx op
-  | CBinOpL op C e2 => rec C $ BinOpLCtx op e2
-  | CBinOpR op e1 C => recv e1 C $ BinOpRCtx op
-  | CIf C e1 e2 => rec C $ IfCtx e1 e2
-  | CPairL C e2 => rec C $ PairLCtx e2
-  | CPairR e1 C => recv e1 C PairRCtx
-  | CFst C => rec C FstCtx
-  | CSnd C => rec C SndCtx
-  | CInjL C => rec C InjLCtx
-  | CInjR C => rec C InjRCtx
-  | CCase C e1 e2 => rec C $ CaseCtx e1 e2
-  | CAssert C => rec C AssertCtx
-  | CAlloc C => rec C AllocCtx
-  | CLoad C => rec C LoadCtx
-  | CStoreL C e2 => rec C $ StoreLCtx e2
-  | CStoreR e1 C => recv e1 C StoreRCtx
-  | CCASL C e1 e2 => rec C $ CasLCtx e1 e2
-  | CCASM e0 C e2 => v0 ← to_val e0; rec C $ CasMCtx v0 e2
-  | CCASR e0 e1 C => v0 ← to_val e0; v1 ← to_val e1; rec C $ CasRCtx v0 v1
-  | _ => None
-  end.
-
-Lemma to_of_ectx K : to_ectx (of_ectx K) = Some K.
-Proof.
-  elim: K => // Ki K IH. by destruct Ki; simplify_option_eq; repeat f_equal.
-Qed.
-
-Lemma of_to_ectx C K : to_ectx C = Some K → of_ectx K = C.
-Proof.
-  elim: C K; intros; simplify_option_eq; auto using of_to_val with f_equal.
-Qed.
-
-Instance of_ectx_inj : Inj (=) (=) of_ectx.
-Proof. move=>?? EQ. apply (inj Some). by rewrite -!to_of_ectx EQ. Qed.
-
-Lemma to_ectx_fill C K e : to_ectx C = Some K → ctx_fill C e = fill K e.
-Proof.
-  elim: C K; intros; simplify_option_eq;
-    auto using of_to_val, eq_sym with f_equal.
-Qed.
-
-(** * Robust safety *)
-(**
-	Our aim is to show that, under the heap invariant, if we plug
-	a closed, semantically low expression (i.e., verified code)
-	into an adversarial context, the resulting expression is
-	semantically low.
-
-	The proof is by induction on contexts, using the FTLR to zap
-	the context's subexpressions to low values. As in the proof of
-	the FTLR, we must generalize to account for substitution.
-
-	TODO: This is just a special case of the more general result
-	with multi-holed contexts. *That* proof is likely to be
-	shorter, since we can dispense with the FTLR and we'll have
-	fewer cases in the definition of contexts.
- *)
-Section robust_safety.
-  Context `{heapG Σ}.
-  Implicit Types γ : env.
-  Implicit Types C : ctx.
-  Implicit Types e : expr.
-  Implicit Types v : val.
-
-  Definition verified : pbit → expr → iProp Σ := λ p e,
-     (□ (⌜Closed [] e⌝ ∗ WP e @ p; ⊤ {{ low }}))%I.
-
-  Definition safe : ctx → iProp Σ := λ C, (
-    ∀ γ p e, heap_ctx -∗ adv C -∗ low γ -∗ verified p e -∗
-    WP γ (ctx_fill C e) ?{{ low }}
-  )%I.
-
-  Lemma safe_alt C :
-    safe C ⊣⊢
-    ∀ γ p e Φ, heap_ctx -∗ adv C -∗ low γ -∗ verified p e -∗
-    (∀ v, low v -∗ Φ v) -∗ WP γ (ctx_fill C e) ?{{ Φ }}.
-  Proof.
-    iSplit.
-    -  iIntros "Hsafe". iIntros (γ p e Φ) "Hh HC Hγ He".
-      rewrite -wp_wand. by iApply ("Hsafe" with "Hh HC Hγ He").
-    - iIntros "Halt". iIntros (γ p e) "Hh HC Hγ He".
-      iApply ("Halt" with "Hh HC Hγ He []"). by iIntros.
+    rewrite/uPred_valid -compatible_ctx_intro -compatible_spec.
+    by induction c; auto.
   Qed.
 
-  Lemma safe_hole : safe CHole.
+  (**
+	The internal version of [robust_safety]: the expression
+	obtained by plugging an adversarial context with verified code
+	is, under the heap invariant, semantically low.
+  *)
+  Corollary robust_safetyI c es :
+    heap_ctx ⊢ adv_ctx c -∗ ([∗ list] e ∈ es, verified_code e) -∗
+    WP ctx_plug c es ?{{ low }}.
   Proof.
-    iIntros (γ p e) "_ _ _ >(%&He) /=". iApply (wp_forget_progress p).
-    by rewrite substitute_closed.
-  Qed.
-  Hint Extern 1 (_ ⊢ safe CHole) => rewrite -safe_hole.
-
-  Lemma safe_rec f x C : □ safe C -∗ safe (CRec f x C).
-  Proof.
-    (* TODO: Lots of duplication with confined_rec. *)
-    iIntros "#IH". iIntros (γ p e) "#Hh #HC #Hγ #He /=".
-    rewrite adv_ctx substitute_expr. set erec := substitute _ _.
-    case: (decide (Closed (f :b: x :b: []) erec)) => ?;
-      last by iApply wp_stuck_rec_open.
-    iApply wp_value; first exact: to_val_rec.
-    rewrite/erec. set γ' := (delete _ _).
-    iLöb as "Hvrec". rewrite {2}low_val. iAlways. iNext.
-    iIntros (v2) "#Hv2". case: (decide (x = f))=>?.
-    { subst. rewrite -> subst_subst'; last done.	(* ssr rewrite fails *)
-      rewrite of_val_rec subst_substitute; first by rewrite lookup_delete.
-      iApply ("IH" with "Hh HC [] [He]"); last iExact "He".	(* iNext bug *)
-      rewrite insert_delete. iApply (low_env_insert with "Hvrec");
-        first by rewrite lookup_delete.
-      by iApply (low_env_delete with "Hγ"). }
-    rewrite of_val_rec subst_substitute; first by rewrite lookup_delete.
-    rewrite subst_substitute; first by rewrite
-      lookup_insert_ne // lookup_delete_ne // lookup_delete.
-    iApply ("IH" with "Hh HC [] [He]"); last iExact "He".	(* iNext bug *)
-    iApply (low_env_insert with "Hv2"); first by rewrite
-      lookup_insert_ne // lookup_delete_ne // lookup_delete.
-    iApply (low_env_insert with "Hvrec"); first by rewrite
-      lookup_delete.
-    do 2!iApply low_env_delete. iExact "Hγ".
-  Qed.
-  Hint Extern 1 (_ ⊢ safe (CRec _ _ _))
-    => rewrite -safe_rec; exact: always_intro.
-
-  Lemma safe_app_l C1 e2 : safe C1 -∗ safe (CAppL C1 e2).
-  Proof.
-    iIntros "IH". iIntros (γ p e) "#Hh Happ #Hγ He /=".
-    rewrite adv_ctx substitute_expr. iDestruct "Happ" as "(HC1&He2)".
-    iApply (wp_on_val_app_bind with "[-He2]").
-    - by iApply ("IH" with "Hh HC1 Hγ He").
-    - by iApply (ftlr with "Hh Hγ He2").
-  Qed.
-  Hint Extern 1 (_ ⊢ safe (CAppL _ _)) => rewrite -safe_app_l.
-
-  Lemma safe_app_r e1 C2 : safe C2 -∗ safe (CAppR e1 C2).
-  Proof.
-    iIntros "IH". iIntros (γ p e) "#Hh Happ #Hγ He /=".
-    rewrite adv_ctx substitute_expr. iDestruct "Happ" as "(He1&HC2)".
-    wp_apply (wp_on_val_app_bind with "[He1]").
-    - by iApply (ftlr with "Hh Hγ He1").
-    - by iApply ("IH" with "Hh HC2 Hγ He").
-  Qed.
-  Hint Extern 1 (_ ⊢ safe (CAppR _ _)) => rewrite -safe_app_r.
-
-  Lemma safe_un_op op C : safe C -∗ safe (CUnOp op C).
-  Proof.
-    iIntros "IH". iIntros (γ p e) "Hh HC Hγ He /=".
-    rewrite adv_ctx substitute_expr.
-    iApply wp_on_val_un_op_bind. by iApply ("IH" with "Hh HC Hγ He").
-  Qed.
-  Hint Extern 1 (_ ⊢ safe (CUnOp _ _)) => rewrite -safe_un_op.
-
-  Lemma safe_bin_op_l op C1 e2 : safe C1 -∗ safe (CBinOpL op C1 e2).
-  Proof.
-    iIntros "IH". iIntros (γ p e) "#Hh Hop #Hγ He /=".
-    rewrite adv_ctx substitute_expr. iDestruct "Hop" as "(HC1&He2)".
-    iApply (wp_on_val_bin_op_bind with "[-He2]").
-    - by iApply ("IH" with "Hh HC1 Hγ He").
-    - by iApply (ftlr with "Hh Hγ He2").
-  Qed.
-  Hint Extern 1 (_ ⊢ safe (CBinOpL _ _ _)) => rewrite -safe_bin_op_l.
-
-  Lemma safe_bin_op_r op e1 C2 : safe C2 -∗ safe (CBinOpR op e1 C2).
-  Proof.
-    iIntros "IH". iIntros (γ p e) "#Hh Hop #Hγ He /=".
-    rewrite adv_ctx substitute_expr. iDestruct "Hop" as "(He1&HC2)".
-    iApply (wp_on_val_bin_op_bind with "[He1]").
-    - by iApply (ftlr with "Hh Hγ He1").
-    - by iApply ("IH" with "Hh HC2 Hγ He").
-  Qed.
-  Hint Extern 1 (_ ⊢ safe (CBinOpR _ _ _)) => rewrite -safe_bin_op_r.
-
-  Lemma safe_if C e1 e2 : safe C -∗ safe (CIf C e1 e2).
-  Proof.
-    iIntros "IH". iIntros (γ p e) "#Hh Hif #Hγ He /=".
-    rewrite adv_ctx substitute_expr. iDestruct "Hif" as "(HC&He1&He2)".
-    wp_apply (wp_any_if_bind with "[-He1 He2]"); last iSplit.
-    - by iApply ("IH" with "Hh HC Hγ He").
-    - by iApply (ftlr with "Hh Hγ He1").
-    - by iApply (ftlr with "Hh Hγ He2").
-  Qed.
-  Hint Extern 1 (_ ⊢ safe (CIf _ _ _)) => rewrite -safe_if.
-
-  Lemma safe_if_l e0 C1 e2 : safe C1 -∗ safe (CIfL e0 C1 e2).
-  Proof.
-    iIntros "IH". iIntros (γ p e) "#Hh Hif #Hγ He /=".
-    rewrite adv_ctx substitute_expr. iDestruct "Hif" as "(He0&HC&He2)".
-    wp_apply (wp_any_if_bind with "[He0]"); last iSplit.
-    - by iApply (ftlr with "Hh Hγ He0").
-    - by iApply ("IH" with "Hh HC Hγ He").
-    - by iApply (ftlr with "Hh Hγ He2").
-  Qed.
-  Hint Extern 1 (_ ⊢ safe (CIfL _ _ _)) => rewrite -safe_if_l.
-
-  Lemma safe_if_r e0 e1 C2 : safe C2 -∗ safe (CIfR e0 e1 C2).
-  Proof.
-    iIntros "IH". iIntros (γ p e) "#Hh Hif #Hγ He /=".
-    rewrite adv_ctx substitute_expr. iDestruct "Hif" as "(He0&He1&HC)".
-    wp_apply (wp_any_if_bind with "[He0]"); last iSplit.
-    - by iApply (ftlr with "Hh Hγ He0").
-    - by iApply (ftlr with "Hh Hγ He1").
-    - by iApply ("IH" with "Hh HC Hγ He").
-  Qed.
-  Hint Extern 1 (_ ⊢ safe (CIfR _ _ _)) => rewrite -safe_if_r.
-
-  Lemma safe_pair_l C1 e2 : safe C1 -∗ safe (CPairL C1 e2).
-  Proof.
-    iIntros "IH". iIntros (γ p e) "#Hh Hp #Hγ He /=".
-    rewrite adv_ctx substitute_expr. iDestruct "Hp" as "(HC1&He2)".
-    wp_apply (wp_on_val_pair_bind with "[-He2]").
-    - by iApply ("IH" with "Hh HC1 Hγ He").
-    - by iApply (ftlr with "Hh Hγ He2").
-  Qed.
-  Hint Extern 1 (_ ⊢ safe (CPairL _ _)) => rewrite -safe_pair_l.
-
-  Lemma safe_pair_r e1 C2 : safe C2 -∗ safe (CPairR e1 C2).
-  Proof.
-    iIntros "IH". iIntros (γ p e) "#Hh Hp #Hγ He /=".
-    rewrite adv_ctx substitute_expr. iDestruct "Hp" as "(He1&HC2)".
-    wp_apply (wp_on_val_pair_bind with "[He1]").
-    - by iApply (ftlr with "Hh Hγ He1").
-    - by iApply ("IH" with "Hh HC2 Hγ He").
-  Qed.
-  Hint Extern 1 (_ ⊢ safe (CPairR _ _)) => rewrite -safe_pair_r.
-
-  Lemma safe_fst C : safe C -∗ safe (CFst C).
-  Proof.
-    iIntros "IH". iIntros (γ p e) "Hh HC Hγ He /=".
-    rewrite adv_ctx substitute_expr.
-    wp_apply wp_on_val_fst_bind. by iApply ("IH" with "Hh HC Hγ He").
-  Qed.
-  Hint Extern 1 (_ ⊢ safe (CFst _)) => rewrite -safe_fst.
-
-  Lemma safe_snd C : safe C -∗ safe (CSnd C).
-  Proof.
-    iIntros "IH". iIntros (γ p e) "Hh HC Hγ He /=".
-    rewrite adv_ctx substitute_expr.
-    wp_apply wp_on_val_snd_bind. by iApply ("IH" with "Hh HC Hγ He").
-  Qed.
-  Hint Extern 1 (_ ⊢ safe (CSnd _)) => rewrite -safe_snd.
-
-  Lemma safe_inl C : safe C -∗ safe (CInjL C).
-  Proof.
-    iIntros "IH". iIntros (γ p e) "Hh HC Hγ He /=".
-    rewrite adv_ctx substitute_expr.
-    wp_apply wp_on_val_inl_bind. by iApply ("IH" with "Hh HC Hγ He").
-  Qed.
-  Hint Extern 1 (_ ⊢ safe (CInjL _)) => rewrite -safe_inl.
-
-  Lemma safe_inr C : safe C -∗ safe (CInjR C).
-  Proof.
-    iIntros "IH". iIntros (γ p e) "Hh HC Hγ He /=".
-    rewrite adv_ctx substitute_expr.
-    wp_apply wp_on_val_inr_bind. by iApply ("IH" with "Hh HC Hγ He").
-  Qed.
-  Hint Extern 1 (_ ⊢ safe (CInjR _)) => rewrite -safe_inr.
-
-  Lemma safe_case C e1 e2 : safe C -∗ safe (CCase C e1 e2).
-  Proof.
-    iIntros "IH". iIntros (γ p e) "#Hh Hc #Hγ He /=".
-    rewrite adv_ctx substitute_expr. iDestruct "Hc" as "(HC&He1&He2)".
-    wp_apply (wp_on_val_case_bind with "[-He1 He2]");
-      last (iIntros (v0) "Hv0"; iSplit; wp_bind (γ _)).
-    - by iApply ("IH" with "Hh HC Hγ He").
-    - iApply (ftlr_alt with "Hh Hγ He1"). iIntros (f) "Hf".
-      by iApply (wp_on_val_app_bind with "[Hf] [Hv0]"); wp_value.
-    - iApply (ftlr_alt with "Hh Hγ He2"). iIntros (f) "Hf".
-      by iApply (wp_on_val_app_bind with "[Hf] [Hv0]"); wp_value.
-  Qed.
-  Hint Extern 1 (_ ⊢ safe (CCase _ _ _)) => rewrite -safe_case.
-
-  Lemma safe_case_l e0 C1 e2 : safe C1 -∗ safe (CCaseL e0 C1 e2).
-  Proof.
-    iIntros "IH". iIntros (γ p e) "#Hh Hc #Hγ He /=".
-    rewrite adv_ctx substitute_expr. iDestruct "Hc" as "(He0&HC&He2)".
-    wp_apply (wp_on_val_case_bind with "[He0]");
-      last (iIntros (v0) "Hv0"; iSplit; wp_bind (γ _)).
-    - by iApply (ftlr with "Hh Hγ He0").
-    - rewrite safe_alt. iApply ("IH" with "Hh HC Hγ He"). iIntros (f) "Hf".
-      by iApply (wp_on_val_app_bind with "[Hf] [Hv0]"); wp_value.
-    - iApply (ftlr_alt with "Hh Hγ He2"). iIntros (f) "Hf".
-      by iApply (wp_on_val_app_bind with "[Hf] [Hv0]"); wp_value.
-  Qed.
-  Hint Extern 1 (_ ⊢ safe (CCaseL _ _ _)) => rewrite -safe_case_l.
-
-  Lemma safe_case_r e0 e1 C2 : safe C2 -∗ safe (CCaseR e0 e1 C2).
-  Proof.
-    iIntros "IH". iIntros (γ p e) "#Hh Hc #Hγ He /=".
-    rewrite adv_ctx substitute_expr. iDestruct "Hc" as "(He0&He1&HC)".
-    wp_apply (wp_on_val_case_bind with "[He0]");
-      last (iIntros (v0) "Hv0"; iSplit; wp_bind (γ _)).
-    - by iApply (ftlr with "Hh Hγ He0").
-    - iApply (ftlr_alt with "Hh Hγ He1"). iIntros (f) "Hf".
-      by iApply (wp_on_val_app_bind with "[Hf] [Hv0]"); wp_value.
-    - rewrite safe_alt. iApply ("IH" with "Hh HC Hγ He"). iIntros (f) "Hf".
-      by iApply (wp_on_val_app_bind with "[Hf] [Hv0]"); wp_value.
-  Qed.
-  Hint Extern 1 (_ ⊢ safe (CCaseR _ _ _)) => rewrite -safe_case_r.
-
-  Lemma safe_assert C : safe (CAssert C).
-  Proof. iIntros (γ p e) "_ Hc _ _ /=". rewrite adv_ctx. by iExFalso. Qed.
-  Hint Extern 1 (_ ⊢ safe (CAssert _)) => rewrite -safe_assert.
-
-  Lemma safe_fork C : safe C -∗ safe (CFork C).
-  Proof.
-    iIntros "IH". iIntros (γ p e) "Hh HC Hγ He /=".
-    rewrite adv_ctx substitute_expr. wp_apply wp_on_val_fork.
-    by iApply ("IH" with "Hh HC Hγ He").
-  Qed.
-  Hint Extern 1 (_ ⊢ safe (CFork _)) => rewrite -safe_fork.
-
-  Lemma safe_alloc C : safe C -∗ safe (CAlloc C).
-  Proof.
-    iIntros "IH". iIntros (γ p e) "#Hh HC Hγ He /=".
-    rewrite adv_ctx substitute_expr.
-    iApply (wp_low_alloc_bind with "Hh"); first done.
-    by iApply ("IH" with "Hh HC Hγ He").
-  Qed.
-  Hint Extern 1 (_ ⊢ safe (CAlloc _)) => rewrite -safe_alloc.
-
-  Lemma safe_load C : safe C -∗ safe (CLoad C).
-  Proof.
-    iIntros "IH". iIntros (γ p e) "#Hh HC Hγ He /=".
-    rewrite adv_ctx substitute_expr.
-    iApply (wp_low_load_bind with "Hh"); first done.
-    by iApply ("IH" with "Hh HC Hγ He").
-  Qed.
-  Hint Extern 1 (_ ⊢ safe (CLoad _)) => rewrite -safe_load.
-
-  Lemma safe_store_l C1 e2 : safe C1 -∗ safe (CStoreL C1 e2).
-  Proof.
-    iIntros "IH". iIntros (γ p e) "#Hh Hp #Hγ He /=".
-    rewrite adv_ctx substitute_expr. iDestruct "Hp" as "(HC1&He2)".
-    iApply (wp_low_store_bind with "Hh [-He2]"); first done.
-    - by iApply ("IH" with "Hh HC1 Hγ He").
-    - by iApply (ftlr with "Hh Hγ He2").
-  Qed.
-  Hint Extern 1 (_ ⊢ safe (CStoreL _ _)) => rewrite -safe_store_l.
-
-  Lemma safe_store_r e1 C2 : safe C2 -∗ safe (CStoreR e1 C2).
-  Proof.
-    iIntros "IH". iIntros (γ p e) "#Hh Hp #Hγ He /=".
-    rewrite adv_ctx substitute_expr. iDestruct "Hp" as "(He1&HC2)".
-    iApply (wp_low_store_bind with "Hh [He1]"); first done.
-    - by iApply (ftlr with "Hh Hγ He1").
-    - by iApply ("IH" with "Hh HC2 Hγ He").
-  Qed.
-  Hint Extern 1 (_ ⊢ safe (CStoreR _ _)) => rewrite -safe_store_r.
-
-  Lemma safe_cas_l C e1 e2 : safe C -∗ safe (CCASL C e1 e2).
-  Proof.
-    iIntros "IH". iIntros (γ p e) "#Hh Hc #Hγ He /=".
-    rewrite adv_ctx substitute_expr. iDestruct "Hc" as "(HC&He1&He2)".
-    wp_apply (wp_low_cas_bind with "Hh [-He1 He2] [He1]"); first done.
-    - by iApply ("IH" with "Hh HC Hγ He").
-    - by iApply (ftlr with "Hh Hγ He1").
-    - by iApply (ftlr with "Hh Hγ He2").
-  Qed.
-  Hint Extern 1 (_ ⊢ safe (CCASL _ _ _)) => rewrite -safe_cas_l.
-
-  Lemma safe_cas_m e0 C1 e2 : safe C1 -∗ safe (CCASM e0 C1 e2).
-  Proof.
-    iIntros "IH". iIntros (γ p e) "#Hh Hc #Hγ He /=".
-    rewrite adv_ctx substitute_expr. iDestruct "Hc" as "(He0&HC&He2)".
-    wp_apply (wp_low_cas_bind with "Hh [He0] [-He2]"); first done.
-    - by iApply (ftlr with "Hh Hγ He0").
-    - by iApply ("IH" with "Hh HC Hγ He").
-    - by iApply (ftlr with "Hh Hγ He2").
-  Qed.
-  Hint Extern 1 (_ ⊢ safe (CCASM _ _ _)) => rewrite -safe_cas_m.
-
-  Lemma safe_cas_r e0 e1 C2 : safe C2 -∗ safe (CCASR e0 e1 C2).
-  Proof.
-    iIntros "IH". iIntros (γ p e) "#Hh Hc #Hγ He /=".
-    rewrite adv_ctx substitute_expr. iDestruct "Hc" as "(He0&He1&HC)".
-    wp_apply (wp_low_cas_bind with "Hh [He0] [He1]"); first done.
-    - by iApply (ftlr with "Hh Hγ He0").
-    - by iApply (ftlr with "Hh Hγ He1").
-    - by iApply ("IH" with "Hh HC Hγ He").
-  Qed.
-  Hint Extern 1 (_ ⊢ safe (CCASR _ _ _)) => rewrite -safe_cas_r.
-
-  Hint Extern 2 =>
-    match goal with
-    | IH : True ⊢ safe ?C |- True ⊢ safe (_ ?C) => rewrite IH
-    end.
-
-  Theorem robust_safetyI' C : safe C.
-  Proof. rewrite/uPred_valid. by induction C; auto. Qed.
-
-  (** The internal version of [robust_safety]. *)
-  Corollary robust_safetyI C γ p e :
-    heap_ctx ⊢ adv C -∗ low γ -∗ verified p e -∗ WP γ (ctx_fill C e) ?{{ low }}.
-  Proof.
-    iIntros "Hh HC Hγ #(% & He)".
-    iApply (robust_safetyI' with "Hh HC Hγ"). by iAlways; iSplit.
+    iIntros "Hh Hadv Hes". setoid_rewrite verified_low.
+    iPoseProof (fundamental_theorem_robust_safety with "Hadv") as "Hc".
+    iSpecialize ("Hc" $! _ with "Hes").
+    iSpecialize ("Hc" $! (∅ : env) with "Hh").
+    by rewrite low_env_empty wand_True substitute_empty.
   Qed.
 End robust_safety.
 
-(** * Adversaries *)
+(** * Fundamental theorem of logical relations. *)
 (**
-	To state the [robust_safety] theorem, we define a special case
-	of adversarial contexts at the meta-level. A _(meta-level)
-	adversary_ is a context containing neither locations nor
-	assertions.
+	The fundamental theorem of logical relations is an easy corollary
+	of the fundamental theorem of robust safety. We just need a few
+	definitions to set it up and a few facts about contexts.
+
+	(We don't actually need this theorem.)
 *)
-Definition AdvExpr : expr → Prop :=
-  fix rec e := match e with
-  | Var _ | Lit _ | Unit => True
-  | Assert _ | Loc _ => False
-  | Rec _ _ e | UnOp _ e | Fst e | Snd e | InjL e | InjR e
-  | Fork e | Alloc e | Load e
-    => rec e
-  | App e1 e2 | BinOp _ e1 e2 | Pair e1 e2 | Store e1 e2 => rec e1 ∧ rec e2
-  | If e1 e2 e3 | Case e1 e2 e3 | CAS e1 e2 e3
-    => rec e1 ∧ rec e2 ∧ rec e3
-  end.
 
-Definition AdvCtx : ctx → Prop :=
-  fix rec C := match C with
-  | CHole => True
-  | CAssert _ => False
-  | CRec _ _ C | CUnOp _ C | CFst C | CSnd C | CInjL C | CInjR C
-  | CFork C | CAlloc C | CLoad C
-    => rec C
-  | CAppL C1 e2 | CBinOpL _ C1 e2 | CPairL C1 e2 | CStoreL C1 e2
-    => rec C1 ∧ AdvExpr e2
-  | CAppR e1 C2 | CBinOpR _ e1 C2 | CPairR e1 C2 | CStoreR e1 C2
-    => AdvExpr e1 ∧ rec C2
-  | CIf C0 e1 e2 | CCase C0 e1 e2 | CCASL C0 e1 e2
-    => rec C0 ∧ AdvExpr e1 ∧ AdvExpr e2
-  | CIfL e0 C1 e2 | CCaseL e0 C1 e2 | CCASM e0 C1 e2
-    => AdvExpr e0 ∧ rec C1 ∧ AdvExpr e2
-  | CIfR e0 e1 C2 | CCaseR e0 e1 C2 | CCASR e0 e1 C2
-    => AdvExpr e0 ∧ AdvExpr e1 ∧ rec C2
-  end.
-
-Section adversary.
+(**
+	An expression is *adversarial* if it contains no assertions
+	and only low locations. (This is a syntactic notion.)
+*)
+Section adv_expr.
   Context `{heapG Σ}.
-  Implicit Types C : ctx.
-  Implicit Types e : expr.
 
-  Lemma adv_expr_i e : AdvExpr e → adv e.
+  Fixpoint adv_expr (e : expr) : iProp Σ :=
+    match e with
+    | Var _ | Lit _ | Unit => True
+    | Assert _ => False
+    | Loc l => low l
+    | Rec _ _ e | UnOp _ e | Fst e | Snd e | InjL e | InjR e
+    | Fork e | Alloc e | Load e
+      => adv_expr e
+    | App e1 e2 | BinOp _ e1 e2 | Pair e1 e2 | Store e1 e2
+      => adv_expr e1 ∗ adv_expr e2
+    | If e1 e2 e3 | Case e1 e2 e3 | CAS e1 e2 e3
+      => adv_expr e1 ∗ adv_expr e2 ∗ adv_expr e3
+    end%I.
+  Global Instance adv_expr_timeless e : TimelessP (adv_expr e).
+  Proof. by elim: e=>//; apply _. Qed.
+  Global Instance adv_expr_persistent e : PersistentP (adv_expr e).
+  Proof. by elim: e=>//; apply _. Qed.
+  Global Instance adv_expr_ne : Proper ((=) ==> dist n) adv_expr.
+  Proof. apply _. Qed.
+  Global Instance adv_expr_proper : Proper ((=) ==> (≡)) adv_expr.
+  Proof. solve_proper. Qed.
+End adv_expr.
+Typeclasses Opaque adv_expr.
+Arguments adv_expr {_ _} !_ / : assert.
+
+Section ftlr.
+  Context `{heapG Σ}.
+
+  (**
+	An expression is *compatible* (with the logical relation
+	underlying low values) if, when it is adversarial, it is also
+	semantically low. Compatibility lifts the syntactic [adv_expr]
+	to the semantic [low_expr].
+  *)
+  Definition compatible_expr : expr → iProp Σ := λ e, (
+    adv_expr e -∗ low_expr e
+  )%I.
+
+  Lemma ctx_plug_of e es : ctx_plug (ctx_of_expr e) es = e.
   Proof.
-    rewrite/uPred_valid.
-    elim: e => //; intros;
-    lazymatch goal with
-    | IH0 : (AdvExpr ?e0 → True ⊢ adv ?e0),
-      IH1 : (AdvExpr ?e1 → True ⊢ adv ?e1),
-      IH2 : (AdvExpr ?e2 → True ⊢ adv ?e2),
-      He : (AdvExpr (?f ?e0 ?e1 ?e2)) |- True ⊢ adv (?f ?e0 ?e1 ?e2)
-      => rewrite adv_expr; destruct He as (?&?&?); iSplit; [| iSplit];
-        [by rewrite -IH0 | by rewrite -IH1 | by rewrite -IH2]
-    | IH1 : (AdvExpr ?e1 → True ⊢ adv ?e1),
-      IH2 : (AdvExpr ?e2 → True ⊢ adv ?e2),
-      He : (AdvExpr (?f ?e1 ?e2)) |- True ⊢ adv (?f ?e1 ?e2)
-      => rewrite adv_expr; destruct He as [??]; iSplit;
-        [by rewrite -IH1 | by rewrite -IH2]
+    move: e es.
+    suff ctx_plugM_of e es : ctx_plugM (ctx_of_expr e) es = (e, es).
+    { intros. by rewrite/ctx_plug ctx_plugM_of. }
+    elim: e=>//=; intros;
+    repeat match goal with
+    | H : ctx_plugM ?e ?es = _ |- (ctx_plugM ?e ≫= _) ?es = _ =>
+        rewrite/mbind/plugM_bind H /=; clear H
+    | H : ctx_plugM ?e ?es = _ |- context [ctx_plugM ?e ?es] =>
+        rewrite H; clear H
+    end; reflexivity.
+  Qed.
+  Lemma adv_ctx_of e : adv_expr e -∗ adv_ctx (ctx_of_expr e).
+  Proof.
+    set G := λ e, adv_expr e -∗ adv_ctx (ctx_of_expr e). rewrite -/(G e).
+    elim: e=>//=; intros;
+    match goal with
+    | IH1 : G ?e1, IH2 : G ?e2 |- G (_ ?e1 ?e2) =>
+      iIntros "Hc /="; by rewrite IH1 IH2
+    | IH0 : G ?e0, IH1 : G ?e1, IH2 : G ?e2 |- G (_ ?e0 ?e1 ?e2) =>
+      iIntros "Hc /="; by rewrite IH0 IH1 IH2
     end.
   Qed.
 
-  Lemma adv_ctx_i C : AdvCtx C → adv C.
-  Proof.	(* TODO: Automate. *)
-    elim: C => //=.
-    (* application *)
-    - move=>C1 IH e2 [] ??. rewrite adv_ctx.
-      iSplit. by iApply IH. by iApply adv_expr_i.
-    - move=>e1 C2 IH [] ??. rewrite adv_ctx.
-      iSplit. by iApply adv_expr_i. by iApply IH.
-    (* binary operations *)
-    - move=>op C1 IH e2 [] ??. rewrite adv_ctx.
-      iSplit. by iApply IH. by iApply adv_expr_i.
-    - move=>op e1 C2 IH [] ??. rewrite adv_ctx.
-      iSplit. by iApply adv_expr_i. by iApply IH.
-    (* if *)
-    - move=>C0 IH e1 e2 [] ? [] ??. rewrite adv_ctx.
-      iSplit; [|iSplit]. by iApply IH. by iApply adv_expr_i.
-      by iApply adv_expr_i.
-    - move=>e0 C1 IH e2 [] ? [] ??. rewrite adv_ctx.
-      iSplit; [|iSplit]. by iApply adv_expr_i. by iApply IH.
-      by iApply adv_expr_i.
-    - move=>e0 e1 C2 IH [] ? [] ??. rewrite adv_ctx.
-      iSplit; [|iSplit]. by iApply adv_expr_i. by iApply adv_expr_i.
-      by iApply IH.
-    (* pairing *)
-    - move=>C1 IH e2 [] ??. rewrite adv_ctx.
-      iSplit. by iApply IH. by iApply adv_expr_i.
-    - move=>e1 C2 IH [] ??. rewrite adv_ctx.
-      iSplit. by iApply adv_expr_i. by iApply IH.
-    (* case *)
-    - move=>C0 IH e1 e2 [] ? [] ??. rewrite adv_ctx.
-      iSplit; [|iSplit]. by iApply IH. by iApply adv_expr_i.
-      by iApply adv_expr_i.
-    - move=>e0 C1 IH e2 [] ? [] ??. rewrite adv_ctx.
-      iSplit; [|iSplit]. by iApply adv_expr_i. by iApply IH.
-      by iApply adv_expr_i.
-    - move=>e0 e1 C2 IH [] ? [] ??. rewrite adv_ctx.
-      iSplit; [|iSplit]. by iApply adv_expr_i. by iApply adv_expr_i.
-      by iApply IH.
-    (* store *)
-    - move=>C1 IH e2 [] ??. rewrite adv_ctx.
-      iSplit. by iApply IH. by iApply adv_expr_i.
-    - move=>e1 C2 IH [] ??. rewrite adv_ctx.
-      iSplit. by iApply adv_expr_i. by iApply IH.
-    (* CAS *)
-    - move=>C0 IH e1 e2 [] ? [] ??. rewrite adv_ctx.
-      iSplit; [|iSplit]. by iApply IH. by iApply adv_expr_i.
-      by iApply adv_expr_i.
-    - move=>e0 C1 IH e2 [] ? [] ??. rewrite adv_ctx.
-      iSplit; [|iSplit]. by iApply adv_expr_i. by iApply IH.
-      by iApply adv_expr_i.
-    - move=>e0 e1 C2 IH [] ? [] ??. rewrite adv_ctx.
-      iSplit; [|iSplit]. by iApply adv_expr_i. by iApply adv_expr_i.
-      by iApply IH.
+  Theorem fundamental_theorem_logical_relations e : compatible_expr e.
+  Proof.
+    iIntros "Hadv".
+    iPoseProof (fundamental_theorem_robust_safety (ctx_of_expr e)) as "Hc".
+    rewrite/compatible_ctx -adv_ctx_of. iSpecialize ("Hc" with "Hadv").
+    iSpecialize ("Hc" $! []). by rewrite big_sepL_nil ctx_plug_of wand_True.
   Qed.
-End adversary.
+End ftlr.
